converted to Isar

src/HOL/MiniML/MiniML.thy
@@ -1,12 +1,12 @@
 (* Title:     HOL/MiniML/MiniML.thy
    ID:        $Id$
-   Author:    Wolfgang Naraschewski and Tobias Nipkow
+   Author:    Dieter Nazareth, Wolfgang Naraschewski and Tobias Nipkow
    Copyright  1996 TU Muenchen
 
 Mini_ML with type inference rules.
 *)
 
-MiniML = Generalize + 
+theory MiniML = Generalize:
 
 (* expressions *)
 datatype
@@ -16,17 +16,256 @@ datatype
 consts
         has_type :: "(ctxt * expr * typ)set"
 syntax
-        "@has_type" :: [ctxt, expr, typ] => bool
+        "@has_type" :: "[ctxt, expr, typ] => bool"
                        ("((_) |-/ (_) :: (_))" [60,0,60] 60)
 translations 
         "A |- e :: t" == "(A,e,t):has_type"
 
 inductive has_type
-intrs
-        VarI "[| n < length A; t <| A!n |] ==> A |- Var n :: t"
-        AbsI "[| (mk_scheme t1)#A |- e :: t2 |] ==> A |- Abs e :: t1 -> t2"
-        AppI "[| A |- e1 :: t2 -> t1; A |- e2 :: t2 |] 
-              ==> A |- App e1 e2 :: t1"
-        LETI "[| A |- e1 :: t1; (gen A t1)#A |- e2 :: t |] ==> A |- LET e1 e2 :: t"
+intros
+  VarI: "[| n < length A; t <| A!n |] ==> A |- Var n :: t"
+  AbsI: "[| (mk_scheme t1)#A |- e :: t2 |] ==> A |- Abs e :: t1 -> t2"
+  AppI: "[| A |- e1 :: t2 -> t1; A |- e2 :: t2 |] 
+         ==> A |- App e1 e2 :: t1"
+  LETI: "[| A |- e1 :: t1; (gen A t1)#A |- e2 :: t |] ==> A |- LET e1 e2 :: t"
+
+
+declare has_type.intros [simp]
+declare Un_upper1 [simp] Un_upper2 [simp]
+
+declare is_bound_typ_instance_closed_subst [simp]
+
+
+lemma s'_t_equals_s_t: "!!t::typ. $(%n. if n : (free_tv A) Un (free_tv t) then (S n) else (TVar n)) t = $S t"
+apply (rule typ_substitutions_only_on_free_variables)
+apply (simp add: Ball_def)
+done
+
+declare s'_t_equals_s_t [simp]
+
+lemma s'_a_equals_s_a: "!!A::type_scheme list. $(%n. if n : (free_tv A) Un (free_tv t) then (S n) else (TVar n)) A = $S A"
+apply (rule scheme_list_substitutions_only_on_free_variables)
+apply (simp add: Ball_def)
+done
+
+declare s'_a_equals_s_a [simp]
+
+lemma replace_s_by_s': 
+ "$(%n. if n : (free_tv A) Un (free_tv t) then S n else TVar n) A |-  
+     e :: $(%n. if n : (free_tv A) Un (free_tv t) then S n else TVar n) t  
+  ==> $S A |- e :: $S t"
+
+apply (rule_tac P = "%A. A |- e :: $S t" in ssubst)
+apply (rule s'_a_equals_s_a [symmetric])
+apply (rule_tac P = "%t. $ (%n. if n : free_tv A Un free_tv (?t1 S) then S n else TVar n) A |- e :: t" in ssubst)
+apply (rule s'_t_equals_s_t [symmetric])
+apply simp
+done
+
+lemma alpha_A': "!!A::type_scheme list. $ (%x. TVar (if x : free_tv A then x else n + x)) A = $ id_subst A"
+apply (rule scheme_list_substitutions_only_on_free_variables)
+apply (simp add: id_subst_def)
+done
+
+lemma alpha_A: "!!A::type_scheme list. $ (%x. TVar (if x : free_tv A then x else n + x)) A = A"
+apply (rule alpha_A' [THEN ssubst])
+apply simp
+done
+
+lemma S_o_alpha_typ: "$ (S o alpha) (t::typ) = $ S ($ (%x. TVar (alpha x)) t)"
+apply (induct_tac "t")
+apply (simp_all)
+done
+
+lemma S_o_alpha_typ': "$ (%u. (S o alpha) u) (t::typ) = $ S ($ (%x. TVar (alpha x)) t)"
+apply (induct_tac "t")
+apply (simp_all)
+done
+
+lemma S_o_alpha_type_scheme: "$ (S o alpha) (sch::type_scheme) = $ S ($ (%x. TVar (alpha x)) sch)"
+apply (induct_tac "sch")
+apply (simp_all)
+done
+
+lemma S_o_alpha_type_scheme_list: "$ (S o alpha) (A::type_scheme list) = $ S ($ (%x. TVar (alpha x)) A)"
+apply (induct_tac "A")
+apply (simp_all) 
+apply (rule S_o_alpha_type_scheme [unfolded o_def])
+done
+
+lemma S'_A_eq_S'_alpha_A: "!!A::type_scheme list.  
+      $ (%n. if n : free_tv A Un free_tv t then S n else TVar n) A =  
+      $ ((%x. if x : free_tv A Un free_tv t then S x else TVar x) o  
+         (%x. if x : free_tv A then x else n + x)) A"
+apply (subst S_o_alpha_type_scheme_list)
+apply (subst alpha_A)
+apply (rule refl)
+done
+
+lemma dom_S': 
+ "dom (%n. if n : free_tv A Un free_tv t then S n else TVar n) <=  
+  free_tv A Un free_tv t"
+apply (unfold free_tv_subst dom_def)
+apply (simp (no_asm))
+apply fast
+done
+
+lemma cod_S': 
+  "!!(A::type_scheme list) (t::typ).   
+   cod (%n. if n : free_tv A Un free_tv t then S n else TVar n) <=  
+   free_tv ($ S A) Un free_tv ($ S t)"
+apply (unfold free_tv_subst cod_def subset_def)
+apply (rule ballI)
+apply (erule UN_E)
+apply (drule dom_S' [THEN subsetD])
+apply simp
+apply (fast dest: free_tv_of_substitutions_extend_to_scheme_lists intro: free_tv_of_substitutions_extend_to_types [THEN subsetD])
+done
+
+lemma free_tv_S': 
+ "!!(A::type_scheme list) (t::typ).  
+  free_tv (%n. if n : free_tv A Un free_tv t then S n else TVar n) <=  
+  free_tv A Un free_tv ($ S A) Un free_tv t Un free_tv ($ S t)"
+apply (unfold free_tv_subst)
+apply (fast dest: dom_S' [THEN subsetD] cod_S' [THEN subsetD])
+done
+
+lemma free_tv_alpha: "!!t1::typ.  
+      (free_tv ($ (%x. TVar (if x : free_tv A then x else n + x)) t1) - free_tv A) <=  
+          {x. ? y. x = n + y}"
+apply (induct_tac "t1")
+apply (simp (no_asm))
+apply fast
+apply (simp (no_asm))
+apply fast
+done
+
+lemma aux_plus: "!!(k::nat). n <= n + k"
+apply (induct_tac "k" rule: nat_induct)
+apply (simp (no_asm))
+apply (simp (no_asm_simp))
+done
+
+declare aux_plus [simp]
+
+lemma new_tv_Int_free_tv_empty_type: "!!t::typ. new_tv n t ==> {x. ? y. x = n + y} Int free_tv t = {}"
+apply safe
+apply (cut_tac aux_plus)
+apply (drule new_tv_le)
+apply assumption
+apply (rotate_tac 1)
+apply (drule new_tv_not_free_tv)
+apply fast
+done
+
+lemma new_tv_Int_free_tv_empty_scheme: "!!sch::type_scheme. new_tv n sch ==> {x. ? y. x = n + y} Int free_tv sch = {}"
+apply safe
+apply (cut_tac aux_plus)
+apply (drule new_tv_le)
+apply assumption
+apply (rotate_tac 1)
+apply (drule new_tv_not_free_tv)
+apply fast
+done
+
+lemma new_tv_Int_free_tv_empty_scheme_list: "!A::type_scheme list. new_tv n A --> {x. ? y. x = n + y} Int free_tv A = {}"
+apply (rule allI)
+apply (induct_tac "A")
+apply (simp (no_asm))
+apply (simp (no_asm))
+apply (fast dest: new_tv_Int_free_tv_empty_scheme)
+done
+
+lemma gen_t_le_gen_alpha_t [rule_format (no_asm)]: 
+   "new_tv n A --> gen A t <= gen A ($ (%x. TVar (if x : free_tv A then x else n + x)) t)"
+apply (unfold le_type_scheme_def is_bound_typ_instance)
+apply (intro strip)
+apply (erule exE)
+apply (hypsubst)
+apply (rule_tac x = " (%x. S (if n <= x then x - n else x))" in exI)
+apply (induct_tac "t")
+apply (simp (no_asm))
+apply (case_tac "nat : free_tv A")
+apply (simp (no_asm_simp))
+apply (subgoal_tac "n <= n + nat")
+apply (drule new_tv_le)
+apply assumption
+apply (drule new_tv_not_free_tv)
+apply (drule new_tv_not_free_tv)
+apply (simp (no_asm_simp) add: diff_add_inverse)
+apply (simp (no_asm))
+apply (simp (no_asm_simp))
+done
+
+declare has_type.intros [intro!]
+
+lemma has_type_le_env [rule_format (no_asm)]: "A |- e::t ==> !B. A <= B -->  B |- e::t"
+apply (erule has_type.induct)
+   apply (simp (no_asm) add: le_env_def)
+   apply (fastsimp elim: bound_typ_instance_trans)
+  apply simp
+ apply fast
+apply (slow elim: le_env_free_tv [THEN free_tv_subset_gen_le])
+done
+
+(* has_type is closed w.r.t. substitution *)
+lemma has_type_cl_sub: "A |- e :: t ==> !S. $S A |- e :: $S t"
+apply (erule has_type.induct)
+(* case VarI *)
+   apply (rule allI)
+   apply (rule has_type.VarI)
+    apply (simp add: app_subst_list)
+   apply (simp (no_asm_simp) add: app_subst_list)
+  (* case AbsI *)
+  apply (rule allI)
+  apply (simp (no_asm))
+  apply (rule has_type.AbsI)
+  apply simp
+ (* case AppI *)
+ apply (rule allI)
+ apply (rule has_type.AppI)
+  apply simp
+  apply (erule spec)
+ apply (erule spec)
+(* case LetI *)
+apply (rule allI)
+apply (rule replace_s_by_s')
+apply (cut_tac A = "$ S A" and A' = "A" and t = "t" and t' = "$ S t" in ex_fresh_variable)
+apply (erule exE)
+apply (erule conjE)+ 
+apply (rule_tac ?t1.0 = "$ ((%x. if x : free_tv A Un free_tv t then S x else TVar x) o (%x. if x : free_tv A then x else n + x)) t1" in has_type.LETI)
+ apply (drule_tac x = " (%x. if x : free_tv A Un free_tv t then S x else TVar x) o (%x. if x : free_tv A then x else n + x) " in spec)
+ apply (subst S'_A_eq_S'_alpha_A)
+ apply assumption
+apply (subst S_o_alpha_typ)
+apply (subst gen_subst_commutes)
+ apply (rule subset_antisym)
+  apply (rule subsetI)
+  apply (erule IntE)
+  apply (drule free_tv_S' [THEN subsetD])
+  apply (drule free_tv_alpha [THEN subsetD])
+  apply (simp del: full_SetCompr_eq)
+  apply (erule exE)
+  apply (hypsubst)
+  apply (subgoal_tac "new_tv (n + y) ($ S A) ")
+   apply (subgoal_tac "new_tv (n + y) ($ S t) ")
+    apply (subgoal_tac "new_tv (n + y) A")
+     apply (subgoal_tac "new_tv (n + y) t")
+      apply (drule new_tv_not_free_tv)+
+      apply fast
+     apply (rule new_tv_le) prefer 2 apply assumption apply simp
+    apply (rule new_tv_le) prefer 2 apply assumption apply simp
+   apply (rule new_tv_le) prefer 2 apply assumption apply simp
+  apply (rule new_tv_le) prefer 2 apply assumption apply simp
+ apply fast
+apply (rule has_type_le_env)
+ apply (drule spec)
+ apply (drule spec)
+ apply assumption
+apply (rule app_subst_Cons [THEN subst])
+apply (rule S_compatible_le_scheme_lists)
+apply (simp (no_asm_simp))
+done
+
 
 end
