src/HOL/MiniML/Generalize.thy
@@ -6,15 +6,15 @@
 Generalizing type schemes with respect to a context
 *)
 
-Generalize = Instance +
+theory Generalize = Instance:
 
 
 (* gen: binding (generalising) the variables which are not free in the context *)
 
-types ctxt = type_scheme list
+types ctxt = "type_scheme list"
     
 consts
-  gen :: [ctxt, typ] => type_scheme
+  gen :: "[ctxt, typ] => type_scheme"
 
 primrec
   "gen A (TVar n) = (if (n:(free_tv A)) then (FVar n) else (BVar n))"
@@ -23,16 +23,149 @@ primrec
 (* executable version of gen: Implementation with free_tv_ML *)
 
 consts
-  gen_ML_aux :: [nat list, typ] => type_scheme
-
+  gen_ML_aux :: "[nat list, typ] => type_scheme"
 primrec
   "gen_ML_aux A (TVar n) = (if (n: set A) then (FVar n) else (BVar n))"
   "gen_ML_aux A (t1 -> t2) = (gen_ML_aux A t1) =-> (gen_ML_aux A t2)"
 
 consts
-  gen_ML :: [ctxt, typ] => type_scheme
-
+  gen_ML :: "[ctxt, typ] => type_scheme"
 defs
-  gen_ML_def "gen_ML A t == gen_ML_aux (free_tv_ML A) t"
+  gen_ML_def: "gen_ML A t == gen_ML_aux (free_tv_ML A) t"
+
+
+declare equalityE [elim!]
+
+lemma gen_eq_on_free_tv: "free_tv A = free_tv B ==> gen A t = gen B t"
+apply (induct_tac "t")
+apply (simp_all (no_asm_simp))
+done
+
+lemma gen_without_effect [rule_format (no_asm)]: "(free_tv t) <= (free_tv sch) --> gen sch t = (mk_scheme t)"
+apply (induct_tac "t")
+apply (simp (no_asm_simp))
+apply (simp (no_asm))
+apply fast
+done
+
+declare gen_without_effect [simp]
+
+lemma free_tv_gen: "free_tv (gen ($ S A) t) = free_tv t Int free_tv ($ S A)"
+apply (induct_tac "t")
+apply (simp (no_asm))
+apply (case_tac "nat : free_tv ($ S A) ")
+apply (simp (no_asm_simp))
+apply fast
+apply (simp (no_asm_simp))
+apply fast
+apply simp
+apply fast
+done
+
+declare free_tv_gen [simp]
+
+lemma free_tv_gen_cons: "free_tv (gen ($ S A) t # $ S A) = free_tv ($ S A)"
+apply (simp (no_asm))
+apply fast
+done
+
+declare free_tv_gen_cons [simp]
+
+lemma bound_tv_gen: "bound_tv (gen A t1) = (free_tv t1) - (free_tv A)"
+apply (induct_tac "t1")
+apply (simp (no_asm))
+apply (case_tac "nat : free_tv A")
+apply (simp (no_asm_simp))
+apply (simp (no_asm_simp))
+apply fast
+apply (simp (no_asm_simp))
+apply fast
+done
+
+declare bound_tv_gen [simp]
+
+lemma new_tv_compatible_gen [rule_format (no_asm)]: "new_tv n t --> new_tv n (gen A t)"
+apply (induct_tac "t")
+apply auto
+done
+
+lemma gen_eq_gen_ML: "gen A t = gen_ML A t"
+apply (unfold gen_ML_def)
+apply (induct_tac "t")
+ apply (simp (no_asm) add: free_tv_ML_scheme_list)
+apply (simp (no_asm_simp) add: free_tv_ML_scheme_list)
+done
+
+lemma gen_subst_commutes [rule_format (no_asm)]: "(free_tv S) Int ((free_tv t) - (free_tv A)) = {}  
+      --> gen ($ S A) ($ S t) = $ S (gen A t)"
+apply (induct_tac "t")
+ apply (intro strip)
+ apply (case_tac "nat: (free_tv A) ")
+  apply (simp (no_asm_simp))
+ apply simp
+ apply (subgoal_tac "nat ~: free_tv S")
+  prefer 2 apply (fast)
+ apply (simp add: free_tv_subst dom_def)
+ apply (cut_tac free_tv_app_subst_scheme_list)
+ apply fast
+apply (simp (no_asm_simp))
+apply blast
+done
+
+lemma bound_typ_inst_gen [rule_format (no_asm)]: "free_tv(t::typ) <= free_tv(A) --> bound_typ_inst S (gen A t) = t"
+apply (induct_tac "t")
+apply (simp_all (no_asm_simp))
+apply fast
+done
+declare bound_typ_inst_gen [simp]
+
+lemma gen_bound_typ_instance: 
+  "gen ($ S A) ($ S t) <= $ S (gen A t)"
+apply (unfold le_type_scheme_def is_bound_typ_instance)
+apply safe
+apply (rename_tac "R")
+apply (rule_tac x = " (%a. bound_typ_inst R (gen ($S A) (S a))) " in exI)
+apply (induct_tac "t")
+ apply (simp (no_asm))
+apply (simp (no_asm_simp))
+done
+
+lemma free_tv_subset_gen_le: 
+  "free_tv B <= free_tv A ==> gen A t <= gen B t"
+apply (unfold le_type_scheme_def is_bound_typ_instance)
+apply safe
+apply (rename_tac "S")
+apply (rule_tac x = "%b. if b:free_tv A then TVar b else S b" in exI)
+apply (induct_tac "t")
+ apply (simp (no_asm_simp))
+ apply fast
+apply (simp (no_asm_simp))
+done
+
+lemma gen_t_le_gen_alpha_t [rule_format (no_asm)]: 
+  "new_tv n A -->  
+   gen A t <= gen A ($ (%x. TVar (if x : free_tv A then x else n + x)) t)"
+apply (unfold le_type_scheme_def is_bound_typ_instance)
+apply (intro strip)
+apply (erule exE)
+apply (hypsubst)
+apply (rule_tac x = " (%x. S (if n <= x then x - n else x))" in exI)
+apply (induct_tac "t")
+apply (simp (no_asm))
+apply (case_tac "nat : free_tv A")
+apply (simp (no_asm_simp))
+apply (simp (no_asm_simp))
+apply (subgoal_tac "n <= n + nat")
+apply (frule_tac t = "A" in new_tv_le)
+apply assumption
+apply (drule new_tv_not_free_tv)
+apply (drule new_tv_not_free_tv)
+apply (simp (no_asm_simp) add: diff_add_inverse)
+apply (simp (no_asm) add: le_add1)
+apply (simp (no_asm_simp))
+done
+
+declare gen_t_le_gen_alpha_t [simp]
+
 
 end
