src/HOL/MiniML/Maybe.thy
@@ -6,13 +6,46 @@
 Universal error monad.
 *)
 
-Maybe = Main +
+theory Maybe = Main:
 
 constdefs
-  option_bind :: ['a option, 'a => 'b option] => 'b option
+  option_bind :: "['a option, 'a => 'b option] => 'b option"
   "option_bind m f == case m of None => None | Some r => f r"
 
-syntax "@option_bind" :: [pttrns,'a option,'b] => 'c ("(_ := _;//_)" 0)
+syntax "@option_bind" :: "[pttrns,'a option,'b] => 'c" ("(_ := _;//_)" 0)
 translations "P := E; F" == "option_bind E (%P. F)"
+
+
+(* constructor laws for option_bind *)
+lemma option_bind_Some: "option_bind (Some s) f = (f s)"
+apply (unfold option_bind_def)
+apply (simp (no_asm))
+done
+
+lemma option_bind_None: "option_bind None f = None"
+apply (unfold option_bind_def)
+apply (simp (no_asm))
+done
+
+declare option_bind_Some [simp] option_bind_None [simp]
+
+(* expansion of option_bind *)
+lemma split_option_bind: "P(option_bind res f) =  
+          ((res = None --> P None) & (!s. res = Some s --> P(f s)))"
+apply (unfold option_bind_def)
+apply (rule option.split)
+done
+
+lemma option_bind_eq_None: 
+  "((option_bind m f) = None) = ((m=None) | (? p. m = Some p & f p = None))"
+apply (simp (no_asm) split add: split_option_bind)
+done
+
+declare option_bind_eq_None [simp]
+
+(* auxiliary lemma *)
+lemma rotate_Some: "(y = Some x) = (Some x = y)"
+apply ( simp (no_asm) add: eq_sym_conv)
+done
 
 end
